================================================================================
RESULTADOS DEL ANÁLISIS ROSENFELD-GROEBNER
================================================================================

Número de componentes características: 6


================================================================================
COMPONENTE 1
================================================================================

Ecuación 1:
Eq(u**2, 1 - w**2)

Ecuación 2:
Eq(C**2, (-s*u + D)/c)

Ecuación 3:
Eq(S**2, (-c - s*u + D)/c)

Ecuación 4:
Eq(omega, D**(-2))

Ecuación 5:
Eq(w[y], u)

Ecuación 6:
Eq(D[x], (2*c*C*S*w**2 - 2*c*C*S + s*w[x]*u*w)/(w**2 - 1))

Ecuación 7:
Eq(v1[x], -v2[y])

Ecuación 8:
Eq(v1[y], (v2[x]*D**2 - 1)/D**2)

Ecuación 9:
Eq(vtil1[x], -vtil2[y])

Ecuación 10:
Eq(vtil1[y], vtil2[x] - omegatil)

Ecuación 11:
Eq(omegatil[y, y], (-24*c*nu*s*w[x]*C*S*u*w**3 + 24*c*nu*s*w[x]*C*S*u*w - 24*c*nu*s*u*w**4 + 48*c*nu*s*u*w**2 - 24*c*nu*s*u + 20*c*nu*D*w**4 - 40*c*nu*D*w**2 + 20*c*nu*D - 4*c*C*D*S*v1*w**4 + 8*c*C*D*S*v1*w**2 - 4*c*C*D*S*v1 - 4*c*C*D*S*vtil1*w**4 + 8*c*C*D*S*vtil1*w**2 - 4*c*C*D*S*vtil1 + 6*nu*s**2*w[x]**2*w**4 - 6*nu*s**2*w[x]**2*w**2 + 24*nu*s**2*w**6 - 72*nu*s**2*w**4 + 72*nu*s**2*w**2 - 24*nu*s**2 + 2*nu*s*w[x, x]*D*u*w**3 - 2*nu*s*w[x, x]*D*u*w - 2*nu*s*w[x]**2*D*u + 40*nu*s*D*u*w**4 - 80*nu*s*D*u*w**2 + 40*nu*s*D*u + 2*nu*D[y, y]*D*w**4 - 4*nu*D[y, y]*D*w**2 + 2*nu*D[y, y]*D - 6*nu*D[y]**2*w**4 + 12*nu*D[y]**2*w**2 - 6*nu*D[y]**2 - nu*omegatil[x, x]*D**4*w**4 + 2*nu*omegatil[x, x]*D**4*w**2 - nu*omegatil[x, x]*D**4 - 16*nu*D**2*w**4 + 32*nu*D**2*w**2 - 16*nu*D**2 - 2*s*w[x]*D*u*v1*w**3 + 2*s*w[x]*D*u*v1*w - 2*s*w[x]*D*u*vtil1*w**3 + 2*s*w[x]*D*u*vtil1*w - 2*D[y]*D*v2*w**4 + 4*D[y]*D*v2*w**2 - 2*D[y]*D*v2 - 2*D[y]*D*vtil2*w**4 + 4*D[y]*D*vtil2*w**2 - 2*D[y]*D*vtil2 + omegatil[x]*D**4*v1*w**4 - 2*omegatil[x]*D**4*v1*w**2 + omegatil[x]*D**4*v1 + omegatil[x]*D**4*vtil1*w**4 - 2*omegatil[x]*D**4*vtil1*w**2 + omegatil[x]*D**4*vtil1 + omegatil[y]*D**4*v2*w**4 - 2*omegatil[y]*D**4*v2*w**2 + omegatil[y]*D**4*v2 + omegatil[y]*D**4*vtil2*w**4 - 2*omegatil[y]*D**4*vtil2*w**2 + omegatil[y]*D**4*vtil2)/(nu*D**4*w**4 - 2*nu*D**4*w**2 + nu*D**4))

Ecuación 12:
Eq(v2[y, y], (-4*c*C*S*w**2 + 4*c*C*S - 2*s*w[x]*u*w - v2[x, x]*D**3*w**2 + v2[x, x]*D**3)/(D**3*w**2 - D**3))

Ecuación 13:
Eq(vtil2[y, y], omegatil[x] - vtil2[x, x])


================================================================================
COMPONENTE 2
================================================================================

Ecuación 1:
Eq(nu, 0)

Ecuación 2:
Eq(u**2, 1 - w**2)

Ecuación 3:
Eq(C**2, (-s*u + D)/c)

Ecuación 4:
Eq(S**2, (-c - s*u + D)/c)

Ecuación 5:
Eq(omega, D**(-2))

Ecuación 6:
Eq(w[y], u)

Ecuación 7:
Eq(D[x], (2*c*C*S*w**2 - 2*c*C*S + s*w[x]*u*w)/(w**2 - 1))

Ecuación 8:
Eq(omegatil[y], (4*c*C*S*v1*w**2 - 4*c*C*S*v1 + 4*c*C*S*vtil1*w**2 - 4*c*C*S*vtil1 + 2*s*w[x]*u*v1*w + 2*s*w[x]*u*vtil1*w + 2*D[y]*v2*w**2 - 2*D[y]*v2 + 2*D[y]*vtil2*w**2 - 2*D[y]*vtil2 - omegatil[x]*D**3*v1*w**2 + omegatil[x]*D**3*v1 - omegatil[x]*D**3*vtil1*w**2 + omegatil[x]*D**3*vtil1)/(D**3*v2*w**2 - D**3*v2 + D**3*vtil2*w**2 - D**3*vtil2))

Ecuación 9:
Eq(v1[x], -v2[y])

Ecuación 10:
Eq(v1[y], (v2[x]*D**2 - 1)/D**2)

Ecuación 11:
Eq(vtil1[x], -vtil2[y])

Ecuación 12:
Eq(vtil1[y], vtil2[x] - omegatil)

Ecuación 13:
Eq(v2[y, y], (-4*c*C*S*w**2 + 4*c*C*S - 2*s*w[x]*u*w - v2[x, x]*D**3*w**2 + v2[x, x]*D**3)/(D**3*w**2 - D**3))

Ecuación 14:
Eq(vtil2[y, y], omegatil[x] - vtil2[x, x])


================================================================================
COMPONENTE 3
================================================================================

Ecuación 1:
Eq(nu, 0)

Ecuación 2:
Eq(u**2, 1 - w**2)

Ecuación 3:
Eq(C**2, (-s*u + D)/c)

Ecuación 4:
Eq(S**2, (-c - s*u + D)/c)

Ecuación 5:
Eq(omega, D**(-2))

Ecuación 6:
Eq(vtil2, -v2)

Ecuación 7:
Eq(w[y], u)

Ecuación 8:
Eq(D[x], (2*c*C*S*w**2 - 2*c*C*S + s*w[x]*u*w)/(w**2 - 1))

Ecuación 9:
Eq(omegatil[x], (4*c*C*S*w**2 - 4*c*C*S + 2*s*w[x]*u*w)/(D**3*w**2 - D**3))

Ecuación 10:
Eq(v1[x], -v2[y])

Ecuación 11:
Eq(v1[y], (v2[x]*D**2 - 1)/D**2)

Ecuación 12:
Eq(vtil1[x], v2[y])

Ecuación 13:
Eq(vtil1[y], -v2[x] - omegatil)

Ecuación 14:
Eq(v2[y, y], (-4*c*C*S*w**2 + 4*c*C*S - 2*s*w[x]*u*w - v2[x, x]*D**3*w**2 + v2[x, x]*D**3)/(D**3*w**2 - D**3))
COMPONENTE 6
================================================================================

Ecuación 1:
Eq(c, 0)

Ecuación 2:
Eq(nu, 0)

Ecuación 3:
Eq(u**2, 1 - w**2)

Ecuación 4:
Eq(D, s*u)

Ecuación 5:
Eq(S**2, C**2 - 1)

Ecuación 6:
Eq(omega, -1/(s**2*w**2 - s**2))

Ecuación 7:
Eq(vtil2, -v2)

Ecuación 8:
Eq(w[y], u)

Ecuación 9:
Eq(C[x], S)

Ecuación 10:
Eq(omegatil[x], -2*w[x]*w/(s**2*w**4 - 2*s**2*w**2 + s**2))

Ecuación 11:
Eq(v1[x], -v2[y])

Ecuación 12:
Eq(v1[y], (s**2*v2[x]*w**2 - s**2*v2[x] + 1)/(s**2*w**2 - s**2))

Ecuación 13:
Eq(vtil1[x], v2[y])

Ecuación 14:
Eq(vtil1[y], -v2[x] - omegatil)

Ecuación 15:
Eq(v2[y, y], (-s**2*v2[x, x]*w**4 + 2*s**2*v2[x, x]*w**2 - s**2*v2[x, x] + 2*w[x]*w)/(s**2*w**4 - 2*s**2*w**2 + s**2))